---
title: "Assignment 14"
author: "Michael D'Acampora"
date: "May 12, 2018"
output: html_document
---

This wee, we'll work out some Taylor Series expansions of popular functions.

$f(x) = \frac{1}{1-x}$
$f(x) = e^x$
$f(x) = ln(1+x)$

For each function, only consider its valid ranges as indicated in the notes when you are computing the Taylor Series expansion. Please submit your assignment as a R-Markdown document.

The formula for Taylor Polynomial is:

$$P(x) = \sum_{n=0}^{\infty}\frac{f^{(n)}(c)}{n!}(x-c)^n$$

1. $f(x) = \frac{1}{1-x}$
$$f'(x) = \frac{-1}{(1-x)^2} * -1 = \frac{1}{(1-x)^2} , ~ f'(0) = 1$$
$$f''(x) = \frac{-2}{(1-x)^3} * -1 = \frac{2}{(1-x)^3} , ~ f''(0) = 2$$
$$f'''(x) = \frac{2*-3}{(1-x)^4} * -1 = \frac{6}{(1-x)^4} , ~ f'''(0) = 6$$

The pattern emerging is $f^{(n)}= \frac{n!}{(1-x)^{n+1}}$, which when applied to the Taylor Series definition for x=0 reduces to: $$f(x) = \sum_{n=0}^{\infty}\frac{\frac{n!}{(1-(0))^{n+1}}}{n!}(x)^n = \sum_{n=0}^{\infty} x^n$$

2. $f(x) = e^x$

Since the derivative of $e^x$ is itself, any number of derivations will yield the same result. With that regard, $f^{n}=e^x$. 
Applying the Taylor Series defintion for x=0 gives us:
$$f(x) = \sum_{n=0}^{\infty} \frac{e^{(0)}}{n!}(x)^n = \sum_{n=0}^{\infty} \frac{x^n}{n!}$$

3. $f(x) = ln(1+x)$

$$f'(x) = \frac{1}{1+x},~f'(0)=1$$

$$f''(x) = \frac{-1}{(1+x)^2},~f''(0)=-1$$

$$f'''(x) = \frac{2}{(x+1)^3}, ~f'''(0)=2$$

$$f^{4}(x) = \frac{-6}{(x+1)^4}, ~f^{4}(0)=-6$$
Applying the Taylor Series defintion for x=0 gives us:
$$-\sum_{n=0}^{\infty}(-1)^{n+1}\frac{1}{n}x^n$$